some specs for tensor cores

src/examples/Kuiper.Example.TensorCore.fst
@@ -5,6 +5,8 @@ open Kuiper
 open Kuiper.TensorCore
 open Kuiper.Matrix
 open Kuiper.Matrix.Reprs { row_major, col_major }
+open Kuiper.Spec.GEMM
+open Kuiper.EMatrix
 
 inline_for_extraction noextract
 fn use_wmma_ker
@@ -30,6 +32,14 @@ fn use_wmma_ker
   ()
 }
 
+let matplus_zero_lem (#et:Type) {| scalar et |}
+  (#m #n : nat)
+  (mm : ematrix et m n)
+  : Lemma (requires (forall (x:et). zero `add` x == x))
+          (ensures matplus (const_matrix zero) mm == mm)
+  = assert (equal (matplus (const_matrix zero) mm) mm);
+    ()
+
 [@@CPrologue "__device__";
  CPrologue "inline"]
 fn test
@@ -37,19 +47,30 @@ fn test
   (m2 : gpu_matrix half (row_major 16 16))
   (m3 : gpu_matrix half (row_major 16 16))
   preserves
-    (exists* v. m1 |-> v) **
-    (exists* v. m2 |-> v) **
-    (exists* v. m3 |-> v)
+    m1 |-> 'v1 **
+    m2 |-> 'v2
+  requires
+    m3 |-> 'v3
+  ensures
+    m3 |-> matmul #half 'v1 'v2
 {
-  // let mut fragA : fragment half FragA 16 16 16 FragLRM = magic();
-  let fragA = __alloc_fragment half FragA 16sz 16sz 16sz FragLRM;
-  let fragB = __alloc_fragment half FragB 16sz 16sz 16sz FragLRM;
-  let fragC = __alloc_fragment half FragAccum 16sz 16sz 16sz FragLAccum;
+  let fa = __alloc_fragment half FragA 16sz 16sz 16sz FragLRM;
+  let fb = __alloc_fragment half FragB 16sz 16sz 16sz FragLRM;
+  let fc = __alloc_fragment half FragAccum 16sz 16sz 16sz FragLAccum;
 
-  use_wmma_ker m1 m2 m3 fragA fragB fragC;
+  // use_wmma_ker m1 m2 m3 fragA fragB fragC;
+  mma_loadA fa m1;
+  mma_loadB fb m2;
+  mma_fill fc zero;
+  mma_sync' fa fb fc;
+  mma_store fc m3;
 
-  with x. assert (fragA |-> x); drop_ (fragA |-> x);
-  with x. assert (fragB |-> x); drop_ (fragB |-> x);
-  with x. assert (fragC |-> x); drop_ (fragC |-> x);
+  assume (pure (forall (x:half). zero `add` x == x));
+  matplus_zero_lem (matmul 'v1 'v2);
+  assert m3 |-> matmul 'v1 'v2;
+
+  with x. assert (fa |-> x); drop_ (fa |-> x);
+  with x. assert (fb |-> x); drop_ (fb |-> x);
+  with x. assert (fc |-> x); drop_ (fc |-> x);
   ()
 }
